Mostly fix and majorly simplify step deterministic proof

Semantics/IRStepThms.thy
@@ -83,408 +83,170 @@ qed
 
 subsubsection \<open>Control-flow Step is Deterministic\<close>
 
+inductive_cases StepE[elim]:\<^marker>\<open>tag invisible\<close>
+  "g, p \<turnstile> state \<rightarrow> val"
+
+(*
+definition xor :: "bool \<Rightarrow> bool \<Rightarrow> bool"    (infixl "[+]" 60)
+  where "A [+] B \<equiv> (A \<and> \<not> B) \<or> (\<not> A \<and> B)"
+
+lemma xor_false [simp]:
+  "A [+] False = A"
+  by (simp add: xor_def)
+
+(*lemma xor_true [simp]:
+  "(A [+] B [+] True) = ((A [+] True) \<and> (\<not>B))"
+  by (simp add: xor_def)*)
+
+lemma xor_resolve_true [simp]:
+  "False [+] True = True"
+  by (simp add: xor_def)
+
+lemma xor_unfold [simp]:
+  "A [+] (B [+] C) = A [+] B [+] C"
+  using xor_def by force
+
+definition control_nodes :: "(IRNode \<Rightarrow> bool) list" where
+  "control_nodes = 
+    [is_sequential_node,
+    is_FixedGuardNode,
+    is_BytecodeExceptionNode,
+    is_IfNode,
+    is_AbstractEndNode,
+    is_NewArrayNode,
+    is_ArrayLengthNode,
+    is_LoadIndexedNode,
+    is_StoreIndexedNode,
+    is_NewInstanceNode,
+    is_SignedDivNode,
+    is_SignedRemNode,
+    is_LoadFieldNode,
+    is_StoreFieldNode]"
+
+definition is_control_flow :: "IRNode \<Rightarrow> bool" where
+  "is_control_flow node = fold (\<or>) (map (\<lambda>f. f node) control_nodes) False"
+
+definition control_flow_exclusive :: "IRNode \<Rightarrow> bool" where
+  "control_flow_exclusive node = fold ([+]) (map (\<lambda>f. f node) control_nodes) False"
+
+
+lemma exclusive_control:
+  "is_control_flow n \<Longrightarrow> control_flow_exclusive n"
+  unfolding is_control_flow_def control_flow_exclusive_def
+  control_nodes_def apply simp
+  by (cases n; simp)
+*)
+
+theorem stepDet':
+   "(g, p \<turnstile> state \<rightarrow> next) \<Longrightarrow>
+    (g, p \<turnstile> state \<rightarrow> next') \<Longrightarrow> next = next'"
+proof (induction arbitrary: next' rule: "step.induct")
+  case (SequentialNode nid nid' m h)
+  have notend: "\<not>(is_AbstractEndNode (kind g nid))"
+    by (metis SequentialNode.hyps(1) is_AbstractEndNode.simps is_EndNode.elims(2) is_LoopEndNode_def is_sequential_node.simps(18) is_sequential_node.simps(36))
+  from SequentialNode show ?case apply (elim StepE) using is_sequential_node.simps
+                   apply blast
+                  apply force apply force apply force
+    using notend
+    apply (metis (no_types, lifting) Pair_inject is_AbstractEndNode.simps)
+    by force+
+next
+  case (FixedGuardNode nid cond before "next" condE m val nid' h)
+  then show ?case apply (elim StepE)
+    by force+
+next
+  case (BytecodeExceptionNode nid args st nid' exceptionType h' ref h m' m)
+  then show ?case apply (elim StepE)
+    by force+
+next
+  case (IfNode nid cond tb fb condE m val nid' h)
+  then show ?case apply (elim StepE)
+    apply force+
+    \<comment> \<open>IfNode rule uses expression evaluation\<close>
+    using evalDet repDet apply fastforce
+    by force+
+next
+  case (EndNodes nid merge i phis inps inpsE m vs m' h)
+  have notseq: "\<not>(is_sequential_node (kind g nid))"
+    using EndNodes
+    by (metis is_AbstractEndNode.simps is_EndNode.elims(2) is_LoopEndNode_def is_sequential_node.simps(18) is_sequential_node.simps(36))
+  from EndNodes show ?case apply (elim StepE)
+    using notseq apply force
+                  apply force apply force apply force
+    using indexof_det 
+    unfolding is_AbstractEndNode.simps
+    is_AbstractMergeNode.simps any_usage.simps usages.simps inputs.simps ids_def
+    sorry
+next
+  case (NewArrayNode nid len st nid' lenE m length' arrayType h' ref h refNo h'' m')
+  then show ?case apply (elim StepE) apply force+
+  \<comment> \<open>NewArrayNode rule uses expression evaluation\<close>
+  using evalDet repDet apply fastforce
+  by force+
+next
+  case (ArrayLengthNode nid x nid' xE m ref h arrayVal length' m')
+  then show ?case apply (elim StepE) apply force+
+  \<comment> \<open>ArrayLengthNode rule uses expression evaluation\<close>
+  using evalDet repDet apply fastforce
+  by force+
+next             
+  case (LoadIndexedNode nid index guard array nid' indexE m indexVal arrayE ref h arrayVal loaded m')
+  then show ?case apply (elim StepE) apply force+
+  \<comment> \<open>LoadIndexedNode rule uses expression evaluation\<close>
+  using evalDet repDet
+  apply (metis IRNode.inject(28) Pair_inject Value.inject(2))
+  by force+
+next
+  case (StoreIndexedNode nid check val st index guard array nid' indexE m indexVal arrayE ref valE "value" h arrayVal updated h' m')
+  then show ?case apply (elim StepE) apply force+
+  \<comment> \<open>StoreIndexedNode rule uses expression evaluation\<close>
+    using evalDet repDet
+    apply (metis IRNode.inject(55) Pair_inject Value.inject(2))
+  by force+
+next
+  case (NewInstanceNode nid cname obj nid' h' ref h m' m)
+  then show ?case apply (elim StepE) by force+
+next
+  case (LoadFieldNode nid f obj nid' objE m ref h v m')
+  then show ?case apply (elim StepE) apply force+
+  \<comment> \<open>LoadFieldNode rule uses expression evaluation\<close>
+    using evalDet repDet apply fastforce
+  by force+
+next
+  case (SignedDivNode nid x y zero sb nxt xe ye m v1 v2 v m' h)
+  then show ?case apply (elim StepE) apply force+
+  \<comment> \<open>SignedDivNode rule uses expression evaluation\<close>
+    using evalDet repDet
+    apply (metis IRNode.inject(49) Pair_inject)
+  by force+
+next
+  case (SignedRemNode nid x y zero sb nxt xe ye m v1 v2 v m' h)
+  then show ?case apply (elim StepE) apply force+
+  \<comment> \<open>SignedRemNode rule uses expression evaluation\<close>
+    using evalDet repDet
+    apply (metis IRNode.inject(52) Pair_inject)
+  by force+
+next
+  case (StaticLoadFieldNode nid f nid' h v m' m)
+  then show ?case apply (elim StepE) by force+
+next
+  case (StoreFieldNode nid f newval uu obj nid' newvalE objE m val ref h' h m')
+  then show ?case apply (elim StepE) apply force+
+  \<comment> \<open>StoreFieldNode rule uses expression evaluation\<close>
+    using evalDet repDet
+    apply (metis IRNode.inject(54) Pair_inject Value.inject(2) option.inject)
+  by force+
+next
+  case (StaticStoreFieldNode nid f newval uv nid' newvalE m val h' h m')
+  then show ?case apply (elim StepE) apply force+
+  \<comment> \<open>StaticStoreFieldNode rule uses expression evaluation\<close>
+    using evalDet repDet by fastforce
+qed
+
 theorem stepDet:
    "(g, p \<turnstile> (nid,m,h) \<rightarrow> next) \<Longrightarrow>
    (\<forall> next'. ((g, p \<turnstile> (nid,m,h) \<rightarrow> next') \<longrightarrow> next = next'))"
-proof (induction rule: "step.induct")
-  case (SequentialNode nid "next" m h)
-  have notif: "\<not>(is_IfNode (kind g nid))"
-    by (metis is_IfNode_def SequentialNode.hyps(1) is_sequential_node.simps(22))
-  have notend: "\<not>(is_AbstractEndNode (kind g nid))"
-    by (metis is_AbstractEndNode.simps SequentialNode.hyps(1) is_sequential_node.simps(18,36)
-        is_EndNode.elims(2) is_LoopEndNode_def)
-  have notnew: "\<not>(is_NewInstanceNode (kind g nid))"
-    by (metis is_NewInstanceNode_def SequentialNode.hyps(1) is_sequential_node.simps(42))
-  have notload: "\<not>(is_LoadFieldNode (kind g nid))"
-    by (metis is_LoadFieldNode_def SequentialNode.hyps(1) is_sequential_node.simps(33))
-  have notstore: "\<not>(is_StoreFieldNode (kind g nid))"
-    using is_StoreFieldNode_def SequentialNode.hyps(1)
-    by (metis is_sequential_node.simps(56))
-  have notdivrem:  "\<not>(is_IntegerDivRemNode (kind g nid))"
-    using is_IntegerDivRemNode.simps SequentialNode.hyps(1)
-        is_SignedDivNode_def is_SignedRemNode_def
-    by (metis is_sequential_node.simps(52) is_sequential_node.simps(55))
-  from notif notend notnew notload notstore notdivrem
-  show ?case
-    using SequentialNode Pair_inject
-        step.cases
-    by (smt (verit) IRNode.disc(1718) IRNode.disc(3500) IRNode.disc(926) IRNode.discI(39) is_sequential_node.simps(12) is_sequential_node.simps(14) is_sequential_node.simps(20) is_sequential_node.simps(34) is_sequential_node.simps(41) is_sequential_node.simps(52) is_sequential_node.simps(55) is_sequential_node.simps(57))
-next
-  case (FixedGuardNode nid cond before "next" condE m p val h)
-  have notseq: "\<not>(is_sequential_node (kind g nid))"
-    using is_sequential_node.simps by (simp add: FixedGuardNode.hyps(1))
-  have notend: "\<not>(is_AbstractEndNode (kind g nid))"
-    by (simp add: FixedGuardNode.hyps(1))
-  have notloadindex: "\<not>(is_LoadIndexedNode (kind g nid))"
-    by (simp add: FixedGuardNode.hyps(1))
-  have notstoreindex: "\<not>(is_StoreIndexedNode (kind g nid))"
-    by (simp add: FixedGuardNode.hyps(1))
-  from notseq notend notloadindex notstoreindex
-  show ?case
-    using step.cases Pair_inject FixedGuardNode.hyps(1,5)
-    by (smt (verit) IRNode.disc(1784) IRNode.disc(3566) IRNode.distinct(1511) IRNode.distinct(1535) IRNode.distinct(1557) IRNode.distinct(1559) IRNode.distinct(1579) IRNode.distinct(1585) IRNode.distinct(1589) IRNode.distinct(397) IRNode.distinct(751) IRNode.inject(13))
-
-next
-  case (BytecodeExceptionNode nid args st n' ex h' ref h m' m)
-  have notseq: "\<not>(is_sequential_node (kind g nid))"
-    by (simp add: BytecodeExceptionNode.hyps(1))
-  have notif: "\<not>(is_IfNode (kind g nid))"
-    by (simp add: BytecodeExceptionNode.hyps(1))
-  have notref: "\<not>(is_RefNode (kind g nid))"
-    by (metis notseq is_RefNode_def is_sequential_node.simps(7))
-  have notnew: "\<not>(is_NewInstanceNode (kind g nid))"
-    by (simp add: BytecodeExceptionNode.hyps(1))
-  have notload: "\<not>(is_LoadFieldNode (kind g nid))"
-    by (simp add: BytecodeExceptionNode.hyps(1))
-  have notstore: "\<not>(is_StoreFieldNode (kind g nid))"
-    by (simp add: BytecodeExceptionNode.hyps(1))
-  have notdivrem: "\<not>(is_IntegerDivRemNode (kind g nid))"
-    by (simp add: BytecodeExceptionNode.hyps(1))
-  have notfixedguard: "\<not>(is_FixedGuardNode (kind g nid))"
-    by (simp add: BytecodeExceptionNode.hyps(1))
-  have notend: "\<not>(is_AbstractEndNode (kind g nid))"
-    by (simp add: BytecodeExceptionNode.hyps(1))
-  have notnewarray: "\<not>(is_NewArrayNode (kind g nid))"
-    by (simp add: BytecodeExceptionNode.hyps(1))
-  have notarraylength: "\<not>(is_ArrayLengthNode (kind g nid))"
-    by (simp add: BytecodeExceptionNode.hyps(1))
-  have notloadindex: "\<not>(is_LoadIndexedNode (kind g nid))"
-    by (simp add: BytecodeExceptionNode.hyps(1))
-  have notstoreindex: "\<not>(is_StoreIndexedNode (kind g nid))"
-    by (simp add: BytecodeExceptionNode.hyps(1))
-  from notseq notif notref notnew notload notstore notdivrem notfixedguard notend notnewarray
-       notarraylength notloadindex notstoreindex
-  show ?case
-    by (smt (verit) BytecodeExceptionNode.hyps(1) BytecodeExceptionNode.hyps(2) BytecodeExceptionNode.hyps(3) BytecodeExceptionNode.hyps(4) IRNode.discI(39) IRNode.inject(7) Pair_inject is_ArrayLengthNode_def is_FixedGuardNode_def is_IfNode_def is_IntegerDivRemNode.simps is_LoadFieldNode_def is_LoadIndexedNode_def is_NewArrayNode_def is_SignedDivNode_def is_SignedRemNode_def is_StoreFieldNode_def is_StoreIndexedNode_def step.cases)
-
-next
-  case (IfNode nid cond tb fb m val "next" h)
-  then have notseq: "\<not>(is_sequential_node (kind g nid))"
-    by (simp add: IfNode.hyps(1))
-  have notend: "\<not>(is_AbstractEndNode (kind g nid))"
-    by (simp add: IfNode.hyps(1))
-  have notdivrem: "\<not>(is_IntegerDivRemNode (kind g nid))"
-    by (simp add: IfNode.hyps(1))
-  have notnewarray: "\<not>(is_NewArrayNode (kind g nid))"
-    by (simp add: IfNode.hyps(1))
-  from notseq notend notdivrem notnewarray
-  show ?case
-    using Pair_inject repDet evalDet IfNode.hyps step.cases
-    by (smt (verit) IRNode.disc(2444) IRNode.distinct(1511) IRNode.distinct(1733) IRNode.distinct(1735) IRNode.distinct(1757) IRNode.distinct(1777) IRNode.distinct(1783) IRNode.distinct(1787) IRNode.distinct(1789) IRNode.distinct(401) IRNode.distinct(755) IRNode.inject(15))
-next
-  case (EndNodes nid merge i phis inputs m vs m' h)
-  have notseq: "\<not>(is_sequential_node (kind g nid))"
-    by (metis is_EndNode.elims(2) is_LoopEndNode_def is_sequential_node.simps(18,36)
-        is_AbstractEndNode.simps EndNodes.hyps(1))
-  have notif: "\<not>(is_IfNode (kind g nid))"
-    using is_AbstractEndNode.elims(2) EndNodes.hyps(1) is_IfNode_def
-        is_EndNode.simps(16)
-    by (metis IRNode.distinct_disc(1742))
-  have notref: "\<not>(is_RefNode (kind g nid))"
-    using notseq is_RefNode_def
-    by (metis is_sequential_node.simps(7))
-  have notnew: "\<not>(is_NewInstanceNode (kind g nid))"
-    using is_EndNode.simps(40) is_NewInstanceNode_def
-      is_AbstractEndNode.simps EndNodes.hyps(1)
-    by (metis IRNode.distinct_disc(3053))
-  have notload: "\<not>(is_LoadFieldNode (kind g nid))"
-    using  is_EndNode.simps(28) is_LoadFieldNode_def EndNodes.hyps(1)
-        is_AbstractEndNode.simps
-    by (metis IRNode.distinct_disc(2762))
-  have notstore: "\<not>(is_StoreFieldNode (kind g nid))"
-    using is_EndNode.simps(53) is_StoreFieldNode_def EndNodes.hyps(1)
-      is_AbstractEndNode.simps
-    by (metis IRNode.distinct_disc(3084) is_EndNode.simps(55))
-  have notdivrem: "\<not>(is_IntegerDivRemNode (kind g nid))"
-    using EndNodes.hyps(1) is_SignedDivNode_def is_SignedRemNode_def by force
-  have notfixedguard: "\<not>(is_FixedGuardNode (kind g nid))"
-    using is_EndNode.simps(14) is_FixedGuardNode_def EndNodes.hyps(1)
-        is_AbstractEndNode.simps
-    by (metis IRNode.distinct_disc(1543))
-  have notbytecodeexception: "\<not>(is_BytecodeExceptionNode (kind g nid))"
-    using is_BytecodeExceptionNode_def is_AbstractEndNode.simps
-      is_EndNode.simps(8) EndNodes.hyps(1)
-    by (metis IRNode.distinct_disc(788))
-  have notnewarray: "\<not>(is_NewArrayNode (kind g nid))"
-    using is_EndNode.simps(39) is_NewArrayNode_def EndNodes.hyps(1)
-      is_AbstractEndNode.simps
-    by (metis IRNode.distinct_disc(3052))
-  have notarraylength: "\<not>(is_ArrayLengthNode (kind g nid))"
-    using is_EndNode.simps(5) is_ArrayLengthNode_def EndNodes.hyps(1)
-        is_AbstractEndNode.simps
-    by (metis IRNode.disc(1954))
-  have notloadindex: "\<not>(is_LoadIndexedNode (kind g nid))"
-    using is_EndNode.simps(29) is_LoadIndexedNode_def
-      EndNodes.hyps(1) is_AbstractEndNode.simps
-    by (metis IRNode.disc(1979))
-  have notstoreindex: "\<not>(is_StoreIndexedNode (kind g nid))"
-    using is_EndNode.simps(54) is_AbstractEndNode.simps
-      EndNodes.hyps(1) is_StoreIndexedNode_def
-    by (metis IRNode.distinct_disc(3085) is_EndNode.simps(56))
-  from notseq notif notref notnew notload notstore notdivrem notfixedguard notbytecodeexception
-       notnewarray notarraylength notloadindex notstoreindex
-  show ?case
-    by (smt (verit) is_FixedGuardNode_def repAllDet evalAllDet is_IfNode_def EndNodes step.cases
-        is_RefNode_def Pair_inject is_LoadFieldNode_def is_NewInstanceNode_def is_StoreFieldNode_def
-        is_SignedDivNode_def is_SignedRemNode_def is_IntegerDivRemNode.elims(3) is_NewArrayNode_def
-        is_BytecodeExceptionNode_def is_ArrayLengthNode_def is_LoadIndexedNode_def
-        is_StoreIndexedNode_def)
-next
-  case (NewArrayNode nid len st n' lenE m length' arrayType h' ref h refNo h'')
-  have notseq: "\<not>(is_sequential_node (kind g nid))"
-    by (simp add: NewArrayNode.hyps(1))
-  have notend: "\<not>(is_AbstractEndNode (kind g nid))"
-    by (simp add: NewArrayNode.hyps(1))
-  have notif: "\<not>(is_IfNode (kind g nid))"
-    by (simp add: NewArrayNode.hyps(1))
-  have notload: "\<not>(is_LoadFieldNode (kind g nid))"
-    by (simp add: NewArrayNode.hyps(1))
-  have notstore: "\<not>(is_StoreFieldNode (kind g nid))"
-    by (simp add: NewArrayNode.hyps(1))
-  have notfixedguard: "\<not>(is_FixedGuardNode (kind g nid))"
-    by (simp add: NewArrayNode.hyps(1))
-  have notbytecodeexception: "\<not>(is_BytecodeExceptionNode (kind g nid))"
-    by (simp add: NewArrayNode.hyps(1))
-  have notarraylength: "\<not>(is_ArrayLengthNode (kind g nid))"
-    by (simp add: NewArrayNode.hyps(1))
-  have notnew: "\<not>(is_NewInstanceNode (kind g nid))"
-    by (simp add: NewArrayNode.hyps(1))
-  from notseq notend notif notload notstore notfixedguard notbytecodeexception notarraylength notnew
-  show ?case sledgehammer
-    by (smt (verit) IRNode.disc(1718) IRNode.disc(3500) IRNode.disc(926) IRNode.discI(39) IRNode.distinct(2847) IRNode.distinct(3479) IRNode.distinct(3485) IRNode.distinct(3491) IRNode.inject(38) NewArrayNode.hyps(1) NewArrayNode.hyps(2) NewArrayNode.hyps(3) NewArrayNode.hyps(4) NewArrayNode.hyps(5) NewArrayNode.hyps(6) NewArrayNode.hyps(7) NewArrayNode.hyps(8) Pair_inject Value.inject(2) evalDet is_ArrayLengthNode_def is_BytecodeExceptionNode_def is_FixedGuardNode_def repDet step.cases)
-next
-  case (ArrayLengthNode nid x nid' xE m ref h arrayVal length' m')
-  have notseq: "\<not>(is_sequential_node (kind g nid))"
-    by (simp add: ArrayLengthNode.hyps(1))
-  have notend: "\<not>(is_AbstractEndNode (kind g nid))"
-    by (simp add: ArrayLengthNode.hyps(1))
-  have notif: "\<not>(is_IfNode (kind g nid))"
-    by (simp add: ArrayLengthNode.hyps(1))
-  have notstore: "\<not>(is_StoreFieldNode (kind g nid))"
-    by (simp add: ArrayLengthNode.hyps(1))
-  have notfixedguard: "\<not>(is_FixedGuardNode (kind g nid))"
-    by (simp add: ArrayLengthNode.hyps(1))
-  have notbytecodeexception: "\<not>(is_BytecodeExceptionNode (kind g nid))"
-    by (simp add: ArrayLengthNode.hyps(1))
-  have notnew: "\<not>(is_NewInstanceNode (kind g nid))"
-    by (simp add: ArrayLengthNode.hyps(1))
-  have notnewarray: "\<not>(is_NewArrayNode (kind g nid))"
-    by (simp add: ArrayLengthNode.hyps(1))
-  have notloadindex: "\<not>(is_LoadIndexedNode (kind g nid))"
-    by (simp add: ArrayLengthNode.hyps(1))
-  from notseq notend notif notstore notfixedguard notbytecodeexception notnew notnewarray
-       notloadindex
-  show ?case
-    by (smt (verit) ArrayLengthNode.hyps(1) ArrayLengthNode.hyps(2) ArrayLengthNode.hyps(3) ArrayLengthNode.hyps(4) ArrayLengthNode.hyps(5) ArrayLengthNode.hyps(6) IRNode.disc(1784) IRNode.disc(3500) IRNode.disc(926) IRNode.discI(39) IRNode.distinct(425) IRNode.distinct(469) IRNode.distinct(475) IRNode.distinct(481) IRNode.inject(4) Pair_inject Value.inject(2) evalDet is_BytecodeExceptionNode_def is_FixedGuardNode_def is_NewArrayNode_def repDet step.cases)
-next
-  case (LoadIndexedNode nid index gu array nid' indexE m indexVal arrayE ref h arrayVal loaded m')
-  then have notseq: "\<not>(is_sequential_node (kind g nid))"
-    by simp
-  have notend: "\<not>(is_AbstractEndNode (kind g nid))"
-    by (simp add: LoadIndexedNode.hyps(1))
-  have notif: "\<not>(is_IfNode (kind g nid))"
-    by (simp add: LoadIndexedNode.hyps(1))
-  have notref: "\<not>(is_RefNode (kind g nid))"
-    by (simp add: LoadIndexedNode.hyps(1))
-  have notload: "\<not>(is_LoadFieldNode (kind g nid))"
-    by (simp add: LoadIndexedNode.hyps(1))
-  have notstore: "\<not>(is_StoreFieldNode (kind g nid))"
-    by (simp add: LoadIndexedNode.hyps(1))
-  have notdivrem: "\<not>(is_IntegerDivRemNode (kind g nid))"
-    by (simp add: LoadIndexedNode.hyps(1))
-  have notnewarray: "\<not>(is_NewArrayNode (kind g nid))"
-    by (simp add: LoadIndexedNode.hyps(1))
-  have notarraylength: "\<not>(is_ArrayLengthNode (kind g nid))"
-    by (simp add: LoadIndexedNode.hyps(1))
-  have notstoreindex: "\<not>(is_StoreIndexedNode (kind g nid))"
-    by (simp add: LoadIndexedNode.hyps(1))
-  have notfixedguard: "\<not>(is_FixedGuardNode (kind g nid))"
-    by (simp add: LoadIndexedNode.hyps(1))
-  have notbytecodeexception: "\<not>(is_BytecodeExceptionNode (kind g nid))"
-    by (simp add: LoadIndexedNode.hyps(1))
-  have notnew: "\<not>(is_NewInstanceNode (kind g nid))"
-    by (simp add: LoadIndexedNode.hyps(1))
-  from notseq notend notif notref notload notstore notdivrem notnewarray notarraylength notnew
-       notstoreindex notfixedguard notbytecodeexception
-  show ?case 
-    by (smt (verit) IRNode.disc(1718) IRNode.disc(3500) IRNode.disc(3566) IRNode.disc(926) IRNode.discI(39) IRNode.inject(28) LoadIndexedNode.hyps(1) LoadIndexedNode.hyps(2) LoadIndexedNode.hyps(3) LoadIndexedNode.hyps(4) LoadIndexedNode.hyps(5) LoadIndexedNode.hyps(6) LoadIndexedNode.hyps(7) LoadIndexedNode.hyps(8) Value.inject(2) evalDet is_ArrayLengthNode_def is_BytecodeExceptionNode_def is_FixedGuardNode_def is_IntegerDivRemNode.simps is_NewArrayNode_def is_SignedDivNode_def is_SignedRemNode_def prod.inject repDet step.cases)
-next
-  case (StoreIndexedNode nid ch val st i gu a nid' indexE m iv arrayE ref valE val0 h av new h' m')
-  then have notseq: "\<not>(is_sequential_node (kind g nid))"
-    by simp
-  have notend: "\<not>(is_AbstractEndNode (kind g nid))"
-    by (simp add: StoreIndexedNode.hyps(1))
-  have notif: "\<not>(is_IfNode (kind g nid))"
-    by (simp add: StoreIndexedNode.hyps(1))
-  have notref: "\<not>(is_RefNode (kind g nid))"
-    by (simp add: StoreIndexedNode.hyps(1))
-  have notload: "\<not>(is_LoadFieldNode (kind g nid))"
-    by (simp add: StoreIndexedNode.hyps(1))
-  have notstore: "\<not>(is_StoreFieldNode (kind g nid))"
-    by (simp add: StoreIndexedNode.hyps(1))
-  have notdivrem: "\<not>(is_IntegerDivRemNode (kind g nid))"
-    by (simp add: StoreIndexedNode.hyps(1))
-  have notnewarray: "\<not>(is_NewArrayNode (kind g nid))"
-    by (simp add: StoreIndexedNode.hyps(1))
-  have notarraylength: "\<not>(is_ArrayLengthNode (kind g nid))"
-    by (simp add: StoreIndexedNode.hyps(1))
-  have notfixedguard: "\<not>(is_FixedGuardNode (kind g nid))"
-    by (simp add: StoreIndexedNode.hyps(1))
-  have notbytecodeexception: "\<not>(is_BytecodeExceptionNode (kind g nid))"
-    by (simp add: StoreIndexedNode.hyps(1))
-  have notnew: "\<not>(is_NewInstanceNode (kind g nid))"
-    by (simp add: StoreIndexedNode.hyps(1))
-  from notseq notend notif notref notload notstore notdivrem notnewarray notarraylength notnew
-       notfixedguard notbytecodeexception
-  show ?case
-    by (smt (verit) IRNode.disc(1718) IRNode.disc(3500) IRNode.disc(926) IRNode.discI(39) IRNode.distinct(2881) IRNode.distinct(3931) IRNode.distinct(4009) IRNode.distinct(481) IRNode.inject(55) Pair_inject StoreIndexedNode.hyps(1) StoreIndexedNode.hyps(10) StoreIndexedNode.hyps(11) StoreIndexedNode.hyps(2) StoreIndexedNode.hyps(3) StoreIndexedNode.hyps(4) StoreIndexedNode.hyps(5) StoreIndexedNode.hyps(6) StoreIndexedNode.hyps(7) StoreIndexedNode.hyps(8) StoreIndexedNode.hyps(9) Value.inject(2) evalDet is_BytecodeExceptionNode_def is_FixedGuardNode_def is_NewArrayNode_def repDet step.cases)
-next
-  case (NewInstanceNode nid f obj nxt h' ref h m' m)
-  then have notseq: "\<not>(is_sequential_node (kind g nid))"
-    by simp
-  have notend: "\<not>(is_AbstractEndNode (kind g nid))"
-    by (simp add: NewInstanceNode.hyps(1))
-  have notif: "\<not>(is_IfNode (kind g nid))"
-    by (simp add: NewInstanceNode.hyps(1))
-  have notref: "\<not>(is_RefNode (kind g nid))"
-    by (simp add: NewInstanceNode.hyps(1))
-  have notload: "\<not>(is_LoadFieldNode (kind g nid))"
-    by (simp add: NewInstanceNode.hyps(1))
-  have notstore: "\<not>(is_StoreFieldNode (kind g nid))"
-    by (simp add: NewInstanceNode.hyps(1))
-  have notdivrem:  "\<not>(is_IntegerDivRemNode (kind g nid))"
-    by (simp add: NewInstanceNode.hyps(1))
-  have notnewarray:  "\<not>(is_NewArrayNode (kind g nid))"
-    by (simp add: NewInstanceNode.hyps(1))
-  have notarraylength:  "\<not>(is_ArrayLengthNode (kind g nid))"
-    by (simp add: NewInstanceNode.hyps(1))
-  from notseq notend notif notref notload notstore notdivrem notnewarray notarraylength
-  show ?case
-    using NewInstanceNode step.cases
-        Pair_inject
-    by (smt (verit) IRNode.disc(1718) IRNode.disc(2444) IRNode.disc(3500) IRNode.discI(15) IRNode.discI(4) IRNode.distinct(1559) IRNode.distinct(2849) IRNode.distinct(3529) IRNode.distinct(3535) IRNode.distinct(3541) IRNode.distinct(803) IRNode.inject(39))
-next
-  case (LoadFieldNode nid f obj nxt m ref h v m')
-  then have notseq: "\<not>(is_sequential_node (kind g nid))"
-    by simp
-  have notend: "\<not>(is_AbstractEndNode (kind g nid))"
-    by (simp add: LoadFieldNode.hyps(1))
-  have notdivrem: "\<not>(is_IntegerDivRemNode (kind g nid))"
-    by (simp add: LoadFieldNode.hyps(1))
-  have notif: "\<not>(is_IfNode (kind g nid))"
-    by (simp add: LoadFieldNode.hyps(1))
-  have notref: "\<not>(is_RefNode (kind g nid))"
-    by (simp add: LoadFieldNode.hyps(1))
-  have notstore: "\<not>(is_StoreFieldNode (kind g nid))"
-    by (simp add: LoadFieldNode.hyps(1))
-  have notnewarray: "\<not>(is_NewArrayNode (kind g nid))"
-    by (simp add: LoadFieldNode.hyps(1))
-  have notarraylength: "\<not>(is_ArrayLengthNode (kind g nid))"
-    by (simp add: LoadFieldNode.hyps(1))
-  from notseq notend notdivrem notif notref notstore notnewarray notarraylength
-  show ?case 
-    using LoadFieldNode step.cases evalDet option.discI option.inject
-        Pair_inject repDet Value.inject(2)
-        is_ArrayLengthNode_def is_IfNode_def is_NewArrayNode_def is_StoreFieldNode_def
-    by (smt (verit) IRNode.distinct(1535) IRNode.distinct(2755) IRNode.distinct(2777) IRNode.distinct(2797) IRNode.distinct(2803) IRNode.distinct(2809) IRNode.distinct(779) IRNode.inject(27))
-next
-  case (SignedDivNode nid x y zero sb nxt m v1 v2 v m' h)
-  then have notseq: "\<not>(is_sequential_node (kind g nid))"
-    by simp
-  have notend: "\<not>(is_AbstractEndNode (kind g nid))"
-    by (simp add: SignedDivNode.hyps(1))
-  have notif: "\<not>(is_IfNode (kind g nid))"
-    by (simp add: SignedDivNode.hyps(1))
-  have notref: "\<not>(is_RefNode (kind g nid))"
-    by (simp add: SignedDivNode.hyps(1))
-  have notload: "\<not>(is_LoadFieldNode (kind g nid))"
-    by (simp add: SignedDivNode.hyps(1))
-  have notstore: "\<not>(is_StoreFieldNode (kind g nid))"
-    by (simp add: SignedDivNode.hyps(1))
-  have notnewarray: "\<not>(is_NewArrayNode (kind g nid))"
-    by (simp add: SignedDivNode.hyps(1))
-  have notarraylength: "\<not>(is_ArrayLengthNode (kind g nid))"
-    by (simp add: SignedDivNode.hyps(1))
-  from notseq notend notif notref notload notstore notnewarray notarraylength
-  show ?case
-    using evalDet repDet
-        SignedDivNode Pair_inject is_ArrayLengthNode_def is_IfNode_def is_NewArrayNode_def
-        is_LoadFieldNode_def is_StoreFieldNode_def step.cases
-    by (smt (verit) IRNode.distinct(1579) IRNode.distinct(2869) IRNode.distinct(3529) IRNode.distinct(3925) IRNode.distinct(3931) IRNode.distinct(823) IRNode.inject(49))
-next
-  case (SignedRemNode nid x y zero sb nxt m v1 v2 v m' h)
-  then have notseq: "\<not>(is_sequential_node (kind g nid))"
-    by simp
-  have notend: "\<not>(is_AbstractEndNode (kind g nid))"
-    by (simp add: SignedRemNode.hyps(1))
-  have notif: "\<not>(is_IfNode (kind g nid))"
-    by (simp add: SignedRemNode.hyps(1))
-  have notref: "\<not>(is_RefNode (kind g nid))"
-    by (simp add: SignedRemNode.hyps(1))
-  have notload: "\<not>(is_LoadFieldNode (kind g nid))"
-    by (simp add: SignedRemNode.hyps(1))
-  have notstore: "\<not>(is_StoreFieldNode (kind g nid))"
-    by (simp add: SignedRemNode.hyps(1))
-  have notnewarray: "\<not>(is_NewArrayNode (kind g nid))"
-    by (simp add: SignedRemNode.hyps(1))
-  have notarraylength: "\<not>(is_ArrayLengthNode (kind g nid))"
-    by (simp add: SignedRemNode.hyps(1))
-  have notdivnode: "\<not>(is_SignedDivNode (kind g nid))"
-    by (simp add: SignedRemNode.hyps(1))
-  from notseq notend notif notref notload notstore notnewarray notarraylength notdivnode
-  show ?case 
-    by (smt (verit) IRNode.disc(1718) IRNode.disc(2444) IRNode.disc(3500) IRNode.disc(926) IRNode.distinct(1585) IRNode.distinct(2875) IRNode.distinct(3535) IRNode.distinct(3925) IRNode.distinct(4009) IRNode.distinct(475) IRNode.distinct(829) IRNode.inject(52) SignedRemNode.hyps(1) SignedRemNode.hyps(2) SignedRemNode.hyps(3) SignedRemNode.hyps(4) SignedRemNode.hyps(5) SignedRemNode.hyps(6) SignedRemNode.hyps(7) evalDet prod.inject repDet step.cases)  
-next
-  case (StaticLoadFieldNode nid f nxt h v m' m)
-  then have notseq: "\<not>(is_sequential_node (kind g nid))"
-    by simp
-  have notend: "\<not>(is_AbstractEndNode (kind g nid))"
-    by (simp add: StaticLoadFieldNode.hyps(1))
-  have notdivrem: "\<not>(is_IntegerDivRemNode (kind g nid))"
-    by (simp add: StaticLoadFieldNode.hyps(1))
-  from notseq notend notdivrem
-  show ?case
-    by (smt (verit) IRNode.distinct(1535) IRNode.distinct(1733) IRNode.distinct(2755) IRNode.distinct(2775) IRNode.distinct(2777) IRNode.distinct(2797) IRNode.distinct(2803) IRNode.distinct(2807) IRNode.distinct(2809) IRNode.distinct(425) IRNode.distinct(779) IRNode.inject(27) Pair_inject StaticLoadFieldNode.hyps(1) StaticLoadFieldNode.hyps(2) StaticLoadFieldNode.hyps(3) option.discI step.cases)
-next
-  case (StoreFieldNode nid f newval uu obj nxt m val ref h' h m')
-  then have notseq: "\<not>(is_sequential_node (kind g nid))"
-    by simp
-  have notend: "\<not>(is_AbstractEndNode (kind g nid))"
-    by (simp add: StoreFieldNode.hyps(1))
-  have notdivrem: "\<not>(is_IntegerDivRemNode (kind g nid))"
-    by (simp add: StoreFieldNode.hyps(1))
-  have notif: "\<not>(is_IfNode (kind g nid))"
-    by (simp add: StoreFieldNode.hyps(1))
-  have notref: "\<not>(is_RefNode (kind g nid))"
-    by (simp add: StoreFieldNode.hyps(1))
-  have notload: "\<not>(is_LoadFieldNode (kind g nid))"
-    by (simp add: StoreFieldNode.hyps(1))
-  have notnewarray: "\<not>(is_NewArrayNode (kind g nid))"
-    by (simp add: StoreFieldNode.hyps(1))
-  have notarraylength: "\<not>(is_ArrayLengthNode (kind g nid))"
-    by (simp add: StoreFieldNode.hyps(1))
-  from notseq notend notdivrem notif notref notload notnewarray notarraylength
-  show ?case
-    using  evalDet step.cases repDet
-        StoreFieldNode option.discI Pair_inject Value.inject(2) option.inject
-        is_ArrayLengthNode_def is_IfNode_def is_LoadFieldNode_def is_NewArrayNode_def
-    by (smt (verit) IRNode.distinct(1589) IRNode.distinct(2879) IRNode.distinct(3539) IRNode.distinct(3929) IRNode.distinct(4007) IRNode.distinct(4051) IRNode.distinct(833) IRNode.inject(54))
-
-next
-  case (StaticStoreFieldNode nid f newval uv nxt m val h' h m')
-  then have notseq: "\<not>(is_sequential_node (kind g nid))"
-    by simp
-  have notend: "\<not>(is_AbstractEndNode (kind g nid))"
-    by (simp add: StaticStoreFieldNode.hyps(1))
-  have notdivrem: "\<not>(is_IntegerDivRemNode (kind g nid))"
-    by (simp add: StaticStoreFieldNode.hyps(1))
-  from notseq notend notdivrem
-  show ?case
-    using evalDet
-        IRNode.inject(52) step.cases StoreFieldNode StaticStoreFieldNode.hyps option.distinct(1)
-        Pair_inject repDet
-    by (smt (verit) IRNode.distinct(1589) IRNode.distinct(1787) IRNode.distinct(2807) IRNode.distinct(2879) IRNode.distinct(3489) IRNode.distinct(3539) IRNode.distinct(3929) IRNode.distinct(4007) IRNode.distinct(4051) IRNode.distinct(479) IRNode.distinct(833) IRNode.inject(54))
-qed
+  using stepDet' by simp
 
 lemma stepRefNode:
   "\<lbrakk>kind g nid = RefNode nid'\<rbrakk> \<Longrightarrow> g, p \<turnstile> (nid,m,h) \<rightarrow> (nid',m,h)"
